src/program_proof/mvcc/tuple_write_lock.v
@@ -6,9 +6,9 @@ Context `{!heapGS Σ, !mvcc_ghostG Σ}.
 (*****************************************************************)
 (* func (tuple *Tuple) WriteLock()                               *)
 (*****************************************************************)
-Theorem wp_tuple__WriteLock tuple (tid : u64) (key : u64) γ :
+Theorem wp_tuple__WriteLock tuple (tid : nat) (key : u64) γ :
   is_tuple tuple key γ -∗
-  {{{ mods_token γ key (int.nat tid) }}}
+  {{{ mods_token γ key tid }}}
     Tuple__WriteLock #tuple
   {{{ (phys : list dbval), RET #(); own_tuple_locked tuple key tid phys phys γ }}}.
 Proof.
