src/program_proof/mvcc/wrbuf_update_tuples.v
@@ -8,12 +8,15 @@ Context `{!heapGS Σ, !mvcc_ghostG Σ}.
 (*****************************************************************)
 (* func (wrbuf *WrBuf) UpdateTuples(tid uint64)                  *)
 (*****************************************************************)
-Theorem wp_wrbuf__UpdateTuples wrbuf (tid : u64) mods tpls γ :
-  {{{ own_wrbuf wrbuf mods tpls ∗ own_tuples_updated (int.nat tid) mods tpls γ }}}
+Theorem wp_wrbuf__UpdateTuples wrbuf (tid : u64) sid mods tpls γ :
+  {{{ own_wrbuf wrbuf mods tpls ∗
+      own_tuples_updated (int.nat tid) mods tpls γ ∗
+      active_tid γ tid sid
+  }}}
     WrBuf__UpdateTuples #wrbuf #tid
-  {{{ RET #(); own_wrbuf_xtpls wrbuf mods }}}.
+  {{{ RET #(); own_wrbuf_xtpls wrbuf mods ∗ active_tid γ tid sid }}}.
 Proof.
-  iIntros (Φ) "Hwrbuf HΦ".
+  iIntros (Φ) "(Hwrbuf & Htpls & Hactive) HΦ".
   wp_call.
   iNamed "Hwrbuf".
 
@@ -28,6 +31,77 @@ Proof.
   (*     }                                                   *)
   (* }                                                       *)
   (***********************************************************)
+  wp_loadField.
+  wp_pures.
+  set P :=
+    (λ (i : u64),
+       let mods' := (list_to_map (wrent_to_key_dbval <$> (drop (int.nat i) ents))) in
+       let tpls' := (list_to_map (wrent_to_key_tpl <$> (drop (int.nat i) ents))) in
+       own_tuples_updated (int.nat tid) mods' tpls' γ ∗ active_tid γ tid sid)%I.
+  iDestruct (is_slice_small_acc with "HentsS") as "[HentsS HentsC]".
+  wp_apply (wp_forSlice P with "[] [$HentsS Htpls $Hactive]").
+  { clear Φ.
+    iIntros (i x).
+    iIntros "!>" (Φ) "(HP & %Hbound & %Hlookup) HΦ".
+    subst P. simpl.
+    iDestruct "HP" as "[Htpls Hactive]".
+    apply wrent_to_val_with_lookup in Hlookup as (k & v & w & t & Eqx & Hlookup).
+    subst x.
+    wp_pures.
+    (* Deduce [k ∉ (drop (S (int.nat i)) ents).*1.*1.*1]. *)
+    apply take_drop_middle in Hlookup as Eqents.
+    rewrite -Eqents in HNoDup.
+    do 3 rewrite fmap_app in HNoDup.
+    do 3 rewrite fmap_cons in HNoDup.
+    simpl in HNoDup.
+    apply NoDup_app in HNoDup as (_ & _ & HNoDup).
+    apply NoDup_cons in HNoDup as [Hnotin _].
+    wp_if_destruct.
+    { (* Case [AppendVersion]. *)
+      replace (int.nat (word.add _ _)) with (S (int.nat i)) by word.
+      rewrite (drop_S _ _ _ Hlookup).
+      do 2 rewrite list_to_map_cons.
+      unfold own_tuples_updated. simpl.
+      rewrite big_sepM2_insert; last first.
+      { apply not_elem_of_list_to_map_1. set_solver. }
+      { apply not_elem_of_list_to_map_1. set_solver. }
+      iDestruct "Htpls" as "[[%phys Htpl] Htpls]".
+      wp_apply (wp_tuple__AppendVersion with "[$Hactive $Htpl]").
+      iIntros "Hactive".
+      iApply "HΦ".
+      iFrame.
+    }
+    { (* Case [KillVersion]. *)
+      replace (int.nat (word.add _ _)) with (S (int.nat i)) by word.
+      rewrite (drop_S _ _ _ Hlookup).
+      do 2 rewrite list_to_map_cons.
+      unfold own_tuples_updated. simpl.
+      rewrite big_sepM2_insert; last first.
+      { apply not_elem_of_list_to_map_1. set_solver. }
+      { apply not_elem_of_list_to_map_1. set_solver. }
+      iDestruct "Htpls" as "[[%phys Htpl] Htpls]".
+      wp_apply (wp_tuple__KillVersion with "[$Hactive $Htpl]").
+      iIntros (ret) "Hactive".
+      (* [KillVersion] return a [u64], but the loop body should evaluate to unit. *)
+      admit.
+      (*
+      iApply "HΦ".
+      iFrame.
+      *)
+    }
+  }
+  { subst P. simpl.
+    replace (int.nat 0) with 0%nat by word.
+    rewrite drop_0.
+    by rewrite -Hmods -Htpls.
+  }
+  iIntros "[[_ Hactive] HentsS]".
+  iDestruct ("HentsC" with "HentsS") as "HentsS".
+  wp_pures.
+  iApply "HΦ".
+  iFrame.
+  do 2 iExists _.
+  by iFrame "∗ %".
 Admitted.
 
 End heap.
